lean/Shars/Verification/Rho.lean
@@ -16,21 +16,37 @@ attribute [ext (iff := false)] List.ext_getElem!
 open Aeneas hiding Std.Array
 open Std.alloc.vec
 
-@[progress]
-theorem algos.rho.offset.spec (t : Std.U32)
-: t.val < 24
-→ ∃ output,
-  offset t = .ok output ∧
-  output.val = (@Spec.Keccak.ρ.offset 6 t.val).val
+
+-- TODO: Move this elsewhere
+instance[Inhabited T]: Inhabited (Aeneas.Std.Array T n) where default := ⟨List.replicate n.val default, by simp⟩
+
+@[scalar_tac_simps]
+def Spec.Keccak.ρ.sequence: Array (Fin 5 × Fin 5) := #[(1,0), (0,2), (2,1), (1,2), (2,3), (3,3), (3,0), (0,1), (1,3), (3,1), (1,4), (4,4), (4,0), (0,3), (3,4), (4,3), (3,2), (2,2), (2,0), (0,4), (4,2), (2,4), (4,1), (1,1)]
+@[simp] theorem Spec.Keccak.ρ.size_sequence: ρ.sequence.size = 24 := by simp [sequence]
+
+@[simp] def Spec.Keccak.ρ.sequence.step(t: Nat)
+  (t_succ_idx: t + 1 < 24)
+: let (x,y) := sequence[t]!
+  let (x', y') := sequence[t+1]!
+  x'.val = y.val ∧ y'.val = (2*x + 3*y).val
+:= by simp [Nat.add_lt_iff_lt_sub_right] at t_succ_idx;
+      revert t; native_decide
+
+theorem algos.RHO_OFFSETS.spec'(t: Fin 24)
+: let (x,y) := Spec.Keccak.ρ.sequence[t]!
+  algos.RHO_OFFSETS.val[x]!.val[y]!.val = Spec.Keccak.ρ.offset (l:= 6) t.val
+:= by revert t; native_decide
+
+theorem algos.RHO_OFFSETS.spec(t x y: Nat)
+  (t_idx: t < 24)
+: Spec.Keccak.ρ.sequence[t]!.1.val = x
+→ Spec.Keccak.ρ.sequence[t]!.2.val = y
+→ algos.RHO_OFFSETS.val[x]!.val[y]!.val = Spec.Keccak.ρ.offset (l:= 6) t
 := by
-  intro bounded
-  unfold rho.offset Spec.Keccak.ρ.offset
-  progress* by scalar_tac
-  · calc i.val * i1.val
-    _ ≤ 24 * i1.val := Nat.mul_le_mul_right _ (by scalar_tac)
-    _ ≤ 24 * 25     := Nat.mul_le_mul_left  _ (by scalar_tac)
-    _ ≤ _           := by scalar_tac
-  simp [*, Spec.w]
+  intro x_val y_val
+  have:= algos.RHO_OFFSETS.spec' ⟨t, t_idx⟩
+  simpa [*] using this
+
 
 def IR.rho.bitmangling(state res: List Bool)(x y offset: Nat)(z_start: Nat := 0): List Bool := Id.run do
   let mut res := res
@@ -179,13 +195,20 @@ theorem algos.rho_loop.spec(input res : StateArray) (x y : Std.Usize) (t: Std.U3
 : t.val <= 24
 → x.val < 5
 → y.val < 5
+→ ((h: t.val < 24) → Spec.Keccak.ρ.sequence[t.val]!.1.val = x.val ∧ Spec.Keccak.ρ.sequence[t.val]!.2.val = y.val )
 → ∃ output,
   rho_loop input x y res t = .ok output ∧
   output.toBits = IR.rho.loop input.toBits res.toBits t.val x.val y.val
 := by
-  intro t_lt x_lt y_lt
+  intro t_lt x_lt y_lt sequence_prev
   rw [rho_loop]
   progress*
+  · simp [*]
+    intro t_succ_idx
+    have prev:= sequence_prev (by omega)
+    have:= Spec.Keccak.ρ.sequence.step t (by assumption)
+    simpa [prev, Fin.eq_of_val_eq, Fin.val_add, Fin.val_mul] using this
+
   · simp only [*, Std.Array.toBits]
     simp only [IR.rho.loop, Id.run, Fin.isValue, Id.pure_eq, Id.bind_eq,
       Std.Range.forIn_eq_forIn_range', Std.Range.size, List.forIn_yield_eq_foldl]
@@ -193,7 +216,9 @@ theorem algos.rho_loop.spec(input res : StateArray) (x y : Std.Usize) (t: Std.U3
     simp only [List.range'_advance_left (show 24 - t.val > 0 from by scalar_tac)]
     simp only [Fin.isValue, List.foldl_cons, Fin.val_natCast]
     congr 2
-    · simp [*]
+    · have prev:= sequence_prev (by scalar_tac)
+      have := algos.RHO_OFFSETS.spec t x y (by scalar_tac) prev.left prev.right
+      simp [*]
       apply List.ext_toBits <;> simp [List.length_toBits, IR.rho.length_bitmangling]
       intro x' y' z'
       simp [algos.rho.bitmangling.spec, *]
